src/opt/Reorder.v
@@ -1,0 +1,88 @@
+Require Import Basics.
+Require Import Bool.
+Require Import List.
+
+Require Import sflib.
+Require Import paco.
+Require Import respectful5.
+
+Require Import Basic.
+Require Import Event.
+Require Import Language.
+Require Import Time.
+Require Import Memory.
+Require Import Commit.
+Require Import Thread.
+
+Require Import Configuration.
+Require Import Simulation.
+Require Import Compatibility.
+Require Import MemInv.
+Require Import ReorderBase.
+Require Import ReorderLoad.
+Require Import ReorderStore.
+
+Require Import Syntax.
+Require Import Semantics.
+
+Set Implicit Arguments.
+
+Inductive reorder: forall (i1 i2:Instr.t), Prop :=
+| reorder_intro_load
+    r1 l1 o1 i2
+    (REORDER: reorder_load r1 l1 o1 i2):
+    reorder (Instr.load r1 l1 o1) i2
+| reorder_intro_store
+    l1 v1 o1 i2
+    (REORDER: reorder_store l1 v1 o1 i2):
+    reorder (Instr.store l1 v1 o1) i2
+.
+
+Lemma reorder_sim_stmts
+      i1 i2 (REORDER: reorder i1 i2):
+  sim_stmts eq
+            [Stmt.instr Instr.skip; Stmt.instr i2; Stmt.instr i1]
+            [Stmt.instr i1; Stmt.instr i2]
+            eq.
+Proof.
+  pcofix CIH. ii. subst. pfold. ii. splits.
+  { i. inv TERMINAL_TGT. }
+  { admit. }
+  { i. eexists _, _, _. splits; eauto.
+    inv LOCAL. apply MemInv.sem_bot_inv in PROMISE. rewrite PROMISE. auto.
+  }
+  i. inv STEP_TGT; [|by inv STEP; inv STATE; inv INSTR; inv REORDER].
+  inv STEP; try (inv STATE; inv INSTR; inv REORDER); ss.
+  - (* promise *)
+    exploit sim_local_promise; eauto. i. des.
+    eexists _, _, _, _, _, _. splits; eauto.
+    econs. econs 1; eauto.
+  - (* load *)
+    exploit sim_local_read; eauto. i. des.
+    eexists _, _, _, _, _, _. splits; eauto.
+    + econs. econs 6.
+      { econs. econs. }
+      { s. apply Local.fence_relaxed. apply WF_SRC. }
+    + left. eapply paco7_mon; [apply sim_load_sim_thread|]; ss.
+      econs; eauto.
+  - (* store *)
+    exploit sim_local_write; eauto. i. des.
+    inv STEP_SRC.
+    + eexists _, _, _, _, _, _. splits; eauto.
+      * econs. econs 6.
+        { econs. econs. }
+        { s. apply Local.fence_relaxed. apply WF_SRC. }
+      * left. eapply paco7_mon; [apply sim_store_sim_thread|]; ss.
+        econs; eauto.
+    + exploit Local.add_step_release; try apply ADD; eauto.
+      { inv REORDER0; ss. }
+      i. des.
+      eexists _, _, _, _, _, _. splits.
+      * econs 2; [|econs 1]. econs 6.
+        { econs. econs. }
+        { s. apply Local.fence_relaxed. apply WF_SRC. }
+      * econs. econs 1; eauto.
+      * eauto.
+      * left. eapply paco7_mon; [apply sim_store_sim_thread|]; ss.
+        econs; eauto.
+Admitted.
