src/opt/ReorderBase.v
@@ -1,0 +1,520 @@
+Require Import Basics.
+Require Import Bool.
+Require Import List.
+
+Require Import sflib.
+Require Import paco.
+Require Import respectful5.
+
+Require Import Basic.
+Require Import Event.
+Require Import Language.
+Require Import Time.
+Require Import Memory.
+Require Import Commit.
+Require Import Thread.
+
+Require Import Configuration.
+Require Import Simulation.
+Require Import Compatibility.
+Require Import MemInv.
+
+Require Import Syntax.
+Require Import Semantics.
+
+Set Implicit Arguments.
+
+
+Ltac committac :=
+  repeat
+    (try match goal with
+         | [|- Snapshot.le (Snapshot.join _ _) _] =>
+           apply Snapshot.join_spec
+         | [|- Snapshot.le (Snapshot.incr_reads _ _ _) _] =>
+           apply Snapshot.incr_reads_spec
+         end; ss).  
+
+Lemma reorder_read_read
+      loc1 ts1 val1 released1 ord1
+      loc2 ts2 val2 released2 ord2
+      th0 mem0
+      th1
+      th2
+      (LOC: loc1 <> loc2)
+      (ORD2: Ordering.le ord2 Ordering.release)
+      (WF0: Local.wf th0 mem0)
+      (STEP1: Local.read_step th0 mem0 loc1 ts1 val1 released1 ord1 th1)
+      (STEP2: Local.read_step th1 mem0 loc2 ts2 val2 released2 ord2 th2):
+  exists th1' th2',
+    <<STEP1: Local.read_step th0 mem0 loc2 ts2 val2 released2 ord2 th1'>> /\
+    <<STEP2: Local.read_step th1' mem0 loc1 ts1 val1 released1 ord1 th2'>> /\
+    <<SIM: sim_local th2' th2>>.
+Proof.
+  inv STEP1. inv STEP2.
+  exploit CommitFacts.read_min_spec; try apply WF0; try apply GET0; eauto.
+  { eapply Snapshot.readable_mon; try apply COMMIT0; eauto. apply COMMIT. }
+  i. des.
+  exploit CommitFacts.read_min_spec; try apply WF; try apply GET; eauto.
+  { eapply Snapshot.le_on_readable; eauto. apply COMMIT. }
+  { apply WF0. }
+  i. des.
+  eexists _, _. splits.
+  - econs; eauto.
+  - econs; eauto.
+  - s. econs; s; try apply MemInv.sem_bot.
+    inv COMMIT. inv COMMIT0. inv MONOTONE. inv MONOTONE0.
+    unfold CommitFacts.read_min.
+    destruct (Ordering.le Ordering.acquire ord2) eqn:ORD2'.
+    { destruct ord2; ss. }
+    econs.
+    + destruct (Ordering.le Ordering.acquire ord1) eqn:ORD1; committac.
+      * rewrite ACQUIRE; auto.
+      * rewrite CURRENT1. auto.
+      * rewrite READ1. apply CURRENT2.
+      * rewrite CURRENT1. auto.
+      * rewrite READ1. apply CURRENT2.
+    + ss. i. rewrite RELEASED. auto.
+    + ss. committac.
+      * rewrite ACQUIRABLE. auto.
+      * rewrite ACQUIRABLE1. auto.
+Qed.
+
+Lemma reorder_read_promise
+      loc1 ts1 val1 released1 ord1
+      th0 mem0
+      th1
+      th2 mem2
+      (WF0: Local.wf th0 mem0)
+      (STEP1: Local.read_step th0 mem0 loc1 ts1 val1 released1 ord1 th1)
+      (STEP2: Local.promise_step th1 mem0 th2 mem2):
+  exists th1' th2',
+    <<STEP1: Local.promise_step th0 mem0 th1' mem2>> /\
+    <<STEP2: Local.read_step th1' mem2 loc1 ts1 val1 released1 ord1 th2'>> /\
+    <<LOCAL: sim_local th2' th2>>.
+Proof.
+  inv STEP1. inv STEP2. ss.
+  exploit Memory.promise_future; try apply WF0; eauto. i. des.
+  exploit Commit.future_wf; try apply WF0; eauto. i.
+  exploit Memory.future_get; eauto. i.
+  exploit CommitFacts.read_min_spec; try apply COMMIT; eauto. i. des.
+  eexists _, _. splits.
+  - econs; try reflexivity; try apply MEMORY; eauto.
+  - econs; eauto. s.
+    match goal with
+    | [|- ?x = None] => destruct x eqn:X; auto
+    end.
+    eapply Memory.promise_get_inv in X; try apply MEMORY; try apply WF0; eauto.
+    des; [congruence|]. subst.
+    exploit Memory.promise_get1; try apply MEMORY; try apply WF0; eauto. i.
+    congruence.
+  - s. econs; s; try apply MemInv.sem_bot.
+    rewrite <- COMMIT0. apply CommitFacts.read_min_min. auto.
+Qed.
+
+Lemma reorder_read_fulfill
+      loc1 ts1 val1 released1 ord1
+      loc2 from2 to2 val2 released2 ord2
+      th0 mem0
+      th1
+      th2
+      (LOC: loc1 <> loc2)
+      (ORD: Ordering.le Ordering.sc ord2 -> Ordering.le Ordering.sc ord1 -> False)
+      (WF0: Local.wf th0 mem0)
+      (STEP1: Local.read_step th0 mem0 loc1 ts1 val1 released1 ord1 th1)
+      (STEP2: Local.fulfill_step th1 mem0 loc2 from2 to2 val2 released2 ord2 th2):
+  exists th1' th2',
+    <<STEP1: Local.fulfill_step th0 mem0 loc2 from2 to2 val2 released2 ord2 th1'>> /\
+    <<STEP2: Local.read_step th1' mem0 loc1 ts1 val1 released1 ord1 th2'>> /\
+    <<SIM: sim_local th2' th2>>.
+Proof.
+Admitted.
+
+Lemma reorder_read_write
+      loc1 ts1 val1 released1 ord1
+      loc2 from2 to2 val2 released2 ord2
+      th0 mem0
+      th1 mem1
+      th2
+      (LOC: loc1 <> loc2)
+      (ORD: Ordering.le Ordering.sc ord2 -> Ordering.le Ordering.sc ord1 -> False)
+      (WF0: Local.wf th0 mem0)
+      (STEP1: Local.read_step th0 mem0 loc1 ts1 val1 released1 ord1 th1)
+      (STEP2: Local.write_step th1 mem0 loc2 from2 to2 val2 released2 ord2 th2 mem1):
+  exists th1' th2',
+    <<STEP1: Local.write_step th0 mem0 loc2 from2 to2 val2 released2 ord2 th1' mem1>> /\
+    <<STEP2: Local.read_step th1' mem1 loc1 ts1 val1 released1 ord1 th2'>> /\
+    <<SIM: sim_local th2' th2>>.
+Proof.
+Admitted.
+
+Lemma reorder_read_fence
+      loc1 ts1 val1 released1 ord1
+      ord2
+      th0 mem0
+      th1
+      th2
+      (ORD2: Ordering.le ord2 Ordering.release)
+      (WF0: Local.wf th0 mem0)
+      (STEP1: Local.read_step th0 mem0 loc1 ts1 val1 released1 ord1 th1)
+      (STEP2: Local.fence_step th1 mem0 ord2 th2):
+  exists th1' th2',
+    <<STEP1: Local.fence_step th0 mem0 ord2 th1'>> /\
+    <<STEP2: Local.read_step th1' mem0 loc1 ts1 val1 released1 ord1 th2'>> /\
+    <<SIM: sim_local th2' th2>>.
+Proof.
+Admitted.
+
+Lemma reorder_fulfill_read
+      loc1 from1 to1 val1 released1 ord1
+      loc2 ts2 val2 released2 ord2
+      th0 mem0
+      th1
+      th2
+      (LOC: loc1 <> loc2)
+      (ORD1: Ordering.le ord1 Ordering.acquire)
+      (ORD2: Ordering.le ord2 Ordering.release)
+      (WF0: Local.wf th0 mem0)
+      (STEP1: Local.fulfill_step th0 mem0 loc1 from1 to1 val1 released1 ord1 th1)
+      (STEP2: Local.read_step th1 mem0 loc2 ts2 val2 released2 ord2 th2):
+  exists th1' th2',
+    <<STEP1: Local.read_step th0 mem0 loc2 ts2 val2 released2 ord2 th1'>> /\
+    <<STEP2: Local.fulfill_step th1' mem0 loc1 from1 to1 val1 released1 ord1 th2'>> /\
+    <<SIM: sim_local th2' th2>>.
+Proof.
+Admitted.
+
+Lemma reorder_fulfill_promise
+      loc1 from1 to1 val1 released1 ord1
+      th0 mem0
+      th1
+      th2 mem2
+      (WF0: Local.wf th0 mem0)
+      (STEP1: Local.fulfill_step th0 mem0 loc1 from1 to1 val1 released1 ord1 th1)
+      (STEP2: Local.promise_step th1 mem0 th2 mem2):
+  exists th1' th2',
+    <<STEP1: Local.promise_step th0 mem0 th1' mem2>> /\
+    <<STEP2: Local.fulfill_step th1' mem2 loc1 from1 to1 val1 released1 ord1 th2'>> /\
+    <<LOCAL: sim_local th2' th2>>.
+Proof.
+Admitted.
+
+Lemma reorder_fulfill_fulfill
+      loc1 from1 to1 val1 released1 ord1
+      loc2 from2 to2 val2 released2 ord2
+      th0 mem0
+      th1
+      th2
+      (LOC: loc1 <> loc2)
+      (ORD1: Ordering.le ord1 Ordering.acquire)
+      (WF0: Local.wf th0 mem0)
+      (STEP1: Local.fulfill_step th0 mem0 loc1 from1 to1 val1 released1 ord1 th1)
+      (STEP2: Local.fulfill_step th1 mem0 loc2 from2 to2 val2 released2 ord2 th2):
+  exists th1' th2',
+    <<STEP1: Local.fulfill_step th0 mem0 loc2 from2 to2 val2 released2 ord2 th1'>> /\
+    <<STEP2: Local.fulfill_step th1' mem0 loc1 from1 to1 val1 released1 ord1 th2'>> /\
+    <<SIM: sim_local th2' th2>>.
+Proof.
+Admitted.
+
+Lemma reorder_fulfill_write
+      loc1 from1 to1 val1 released1 ord1
+      loc2 from2 to2 val2 released2 ord2
+      th0 mem0
+      th1
+      th2 mem2
+      (LOC: loc1 <> loc2)
+      (ORD1: Ordering.le ord1 Ordering.acquire)
+      (WF0: Local.wf th0 mem0)
+      (STEP1: Local.fulfill_step th0 mem0 loc1 from1 to1 val1 released1 ord1 th1)
+      (STEP2: Local.write_step th1 mem0 loc2 from2 to2 val2 released2 ord2 th2 mem2):
+  exists th1' th2',
+    <<STEP1: Local.write_step th0 mem0 loc2 from2 to2 val2 released2 ord2 th1' mem2>> /\
+    <<STEP2: Local.fulfill_step th1' mem2 loc1 from1 to1 val1 released1 ord1 th2'>> /\
+    <<SIM: sim_local th2' th2>>.
+Proof.
+Admitted.
+
+Lemma reorder_fence_promise
+      ord1
+      th0 mem0
+      th1
+      th2 mem2
+      (ORD1: Ordering.le ord1 Ordering.acquire)
+      (WF0: Local.wf th0 mem0)
+      (STEP1: Local.fence_step th0 mem0 ord1 th1)
+      (STEP2: Local.promise_step th1 mem0 th2 mem2):
+  exists th1' th2',
+    <<STEP1: Local.promise_step th0 mem0 th1' mem2>> /\
+    <<STEP2: Local.fence_step th1' mem2 ord1 th2'>> /\
+    <<SIM: sim_local th2' th2>>.
+Proof.
+Admitted.
+
+Lemma reorder_fence_fulfill
+      ord1
+      loc2 from2 to2 val2 released2 ord2
+      th0 mem0
+      th1
+      th2
+      (ORD1: Ordering.le ord1 Ordering.acquire)
+      (WF0: Local.wf th0 mem0)
+      (STEP1: Local.fence_step th0 mem0 ord1 th1)
+      (STEP2: Local.fulfill_step th1 mem0 loc2 from2 to2 val2 released2 ord2 th2):
+  exists th1' th2',
+    <<STEP1: Local.fulfill_step th0 mem0 loc2 from2 to2 val2 released2 ord2 th1'>> /\
+    <<STEP2: Local.fence_step th1' mem0 ord1 th2'>> /\
+    <<SIM: sim_local th2' th2>>.
+Proof.
+Admitted.
+
+Lemma reorder_fence_write
+      ord1
+      loc2 from2 to2 val2 released2 ord2
+      th0 mem0
+      th1
+      th2 mem2
+      (ORD1: Ordering.le ord1 Ordering.acquire)
+      (WF0: Local.wf th0 mem0)
+      (STEP1: Local.fence_step th0 mem0 ord1 th1)
+      (STEP2: Local.write_step th1 mem0 loc2 from2 to2 val2 released2 ord2 th2 mem2):
+  exists th1' th2',
+    <<STEP1: Local.write_step th0 mem0 loc2 from2 to2 val2 released2 ord2 th1' mem2>> /\
+    <<STEP2: Local.fence_step th1' mem2 ord1 th2'>> /\
+    <<SIM: sim_local th2' th2>>.
+Proof.
+Admitted.
+
+
+
+
+(* Lemma sim_fulfill_promise *)
+(*       loc from to val released ord *)
+(*       th1_src mem1_src *)
+(*       th1_tgt mem1_tgt *)
+(*       th2_tgt mem2_tgt *)
+(*       (ORD: Ordering.le ord Ordering.relaxed) *)
+(*       (LOCAL1: sim_fulfill loc from to val released ord th1_src th1_tgt) *)
+(*       (MEMORY1: sim_memory mem1_src mem1_tgt) *)
+(*       (WF1_SRC: Local.wf th1_src mem1_src) *)
+(*       (WF1_TGT: Local.wf th1_tgt mem1_tgt) *)
+(*       (STEP_TGT: Local.promise_step th1_tgt mem1_tgt th2_tgt mem2_tgt): *)
+(*   exists th2_src mem2_src, *)
+(*     <<STEP_SRC: Local.promise_step th1_src mem1_src th2_src mem2_src>> /\ *)
+(*     <<LOCAL2: sim_fulfill loc from to val released ord th2_src th2_tgt>> /\ *)
+(*     <<MEMORY2: sim_memory mem2_src mem2_tgt>>. *)
+(* Proof. *)
+(*   inv LOCAL1. inv STEP_TGT. *)
+(*   exploit MemInv.promise; eauto. *)
+(*   { apply WF1_SRC. } *)
+(*   { apply WF1_TGT. } *)
+(*   i. des. *)
+(*   exploit Memory.promise_future; try apply PROMISE_SRC; eauto. *)
+(*   { apply WF1_SRC. } *)
+(*   { apply WF1_SRC. } *)
+(*   i. des. *)
+(*   eexists _, _. splits; eauto. *)
+(*   - econs; eauto. *)
+(*     + reflexivity. *)
+(*     + eapply Commit.future_wf; eauto. apply WF1_SRC. *)
+(*   - econs; s; eauto. etransitivity; eauto. *)
+(* Qed. *)
+
+(* Lemma sim_fulfill_read *)
+(*       loc1 from1 to1 val1 released1 ord1 *)
+(*       loc2 ts2 val2 released2 ord2 *)
+(*       th1_src mem1_src *)
+(*       th1_tgt mem1_tgt *)
+(*       th2_tgt *)
+(*       (LOC: loc1 <> loc2) *)
+(*       (ORD1: Ordering.le ord1 Ordering.relaxed) *)
+(*       (ORD2: Ordering.le ord2 Ordering.release) *)
+(*       (LOCAL1: sim_fulfill loc1 from1 to1 val1 released1 ord1 th1_src th1_tgt) *)
+(*       (MEMORY1: sim_memory mem1_src mem1_tgt) *)
+(*       (WF1_SRC: Local.wf th1_src mem1_src) *)
+(*       (WF1_TGT: Local.wf th1_tgt mem1_tgt) *)
+(*       (STEP_TGT: Local.read_step th1_tgt mem1_tgt loc2 ts2 val2 released2 ord2 th2_tgt): *)
+(*   exists th2_src, *)
+(*     <<STEP_SRC: Local.read_step th1_src mem1_src loc2 ts2 val2 released2 ord2 th2_src>> /\ *)
+(*     <<LOCAL2: sim_fulfill loc1 from1 to1 val1 released1 ord1 th2_src th2_tgt>>. *)
+(* Proof. *)
+(*   inv LOCAL1. inv STEP_TGT. *)
+(*   exploit Memory.le_get. *)
+(*   { apply WF1_SRC. } *)
+(*   { inv PROMISE. eapply Memory.le_get. *)
+(*     - apply Memory.le_join_r. memtac. *)
+(*     - apply Memory.singleton_get. *)
+(*   } *)
+(*   intro GET1_SRC. *)
+(*   exploit Memory.splits_get; try apply GET; eauto. *)
+(*   { apply MEMORY1. } *)
+(*   intro GET2_SRC. *)
+(*   exploit CommitFacts.read_min_spec; try apply GET2_SRC; eauto. *)
+(*   { inv COMMIT. eapply Snapshot.readable_mon; eauto. *)
+(*     etransitivity; [|apply COMMIT2]. apply COMMIT1. *)
+(*   } *)
+(*   { apply WF1_SRC. } *)
+(*   { apply WF1_SRC. } *)
+(*   i. des. *)
+(*   destruct (Ordering.le Ordering.release ord1) eqn:ORD1'. *)
+(*   { destruct ord1; ss. } *)
+(*   assert (RELEASED_SRC: Memory.wf_snapshot released1 mem1_src). *)
+(*   { inv WF1_SRC. inv MEMORY. exploit WF0; try apply GET1_SRC; eauto. } *)
+(*   exploit CommitFacts.write_min_spec; try apply RELEASED_SRC; eauto. *)
+(*   { eapply Snapshot.le_on_writable; eauto. apply COMMIT1. } *)
+(*   { ss. inv COMMIT1. etransitivity; eauto. apply MONOTONE. } *)
+(*   { instantiate (1 := ord1). destruct ord1; ss. } *)
+(*   { apply WF1_SRC. } *)
+(*   i. des. *)
+(*   eexists _. splits; eauto. *)
+(*   - econs; eauto. inv PROMISE. *)
+(*     match goal with *)
+(*     | [|- ?x = None] => destruct x eqn:X; auto *)
+(*     end. *)
+(*     apply Memory.join_get in X; memtac; try congruence. *)
+(*     apply Memory.singleton_get_inv in X. des. congruence. *)
+(*   - econs; eauto. s. *)
+(*     exploit CommitFacts.write_min_min; try apply COMMIT1; eauto. i. *)
+(*     exploit CommitFacts.read_min_min; try apply COMMIT; eauto. i. *)
+(*     unfold CommitFacts.read_min in *. *)
+(*     destruct (Ordering.le Ordering.acquire ord2) eqn:ORD2'. *)
+(*     { destruct ord2; ss. } *)
+(*     inv x0. inv x1. *)
+(*     apply Snapshot.incr_writes_inv in CURRENT1. *)
+(*     apply Snapshot.incr_reads_inv in CURRENT2. des. *)
+(*     econs; ss. *)
+(*     + apply Snapshot.incr_writes_spec. *)
+(*       * apply Snapshot.incr_reads_spec; ss. *)
+(*         etransitivity; [apply COMMIT1|]. *)
+(*         etransitivity; [apply COMMIT2|]. *)
+(*         apply COMMIT. *)
+(*       * etransitivity; [apply COMMIT1|]. *)
+(*         etransitivity; [apply COMMIT2|]. *)
+(*         apply COMMIT. *)
+(*     + i. unfold LocFun.add, LocFun.find. *)
+(*       destruct (Loc.eq_dec loc loc1). *)
+(*       * subst. rewrite ORD1'. *)
+(*         etransitivity; [apply COMMIT1|]. *)
+(*         etransitivity; [apply COMMIT2|]. *)
+(*         apply COMMIT. *)
+(*       * etransitivity; [apply COMMIT1|]. *)
+(*         etransitivity; [apply COMMIT2|]. *)
+(*         apply COMMIT. *)
+(*     + etransitivity; eauto. *)
+(*       apply Snapshot.join_spec. *)
+(*       * apply Snapshot.join_l. *)
+(*       * etransitivity; [|apply Snapshot.join_r]. *)
+(*         etransitivity; [apply COMMIT1|]. *)
+(*         apply COMMIT2. *)
+(* Qed. *)
+
+(* Lemma sim_fulfill_write *)
+(*       loc1 from1 to1 val1 released1 ord1 *)
+(*       loc2 from2 to2 val2 released2 ord2 *)
+(*       th1_src mem1_src *)
+(*       th1_tgt mem1_tgt *)
+(*       th2_tgt mem2_tgt *)
+(*       (LOC: loc1 <> loc2) *)
+(*       (ORD1: Ordering.le ord1 Ordering.relaxed) *)
+(*       (LOCAL1: sim_fulfill loc1 from1 to1 val1 released1 ord1 th1_src th1_tgt) *)
+(*       (MEMORY1: sim_memory mem1_src mem1_tgt) *)
+(*       (WF1_SRC: Local.wf th1_src mem1_src) *)
+(*       (WF1_TGT: Local.wf th1_tgt mem1_tgt) *)
+(*       (STEP_TGT: Local.write_step th1_tgt mem1_tgt loc2 from2 to2 val2 released2 ord2 th2_tgt mem2_tgt): *)
+(*   exists th2_src mem2_src, *)
+(*     <<STEP_SRC: Local.write_step th1_src mem1_src loc2 from2 to2 val2 released2 ord2 th2_src mem2_src>> /\ *)
+(*     <<LOCAL2: sim_fulfill loc1 from1 to1 val1 released1 ord1 th2_src th2_tgt>> /\ *)
+(*     <<MEMORY2: sim_memory mem2_src mem2_tgt>>. *)
+(* Proof. *)
+(*   destruct (Ordering.le Ordering.release ord1) eqn:ORD1'. *)
+(*   { destruct ord1; ss. } *)
+(*   inv LOCAL1. inv STEP_TGT. *)
+(*   exploit MemInv.write; eauto. *)
+(*   { apply WF1_SRC. } *)
+(*   { apply WF1_TGT. } *)
+(*   { inv PROMISE. unfold Memory.join. *)
+(*     unfold Memory.singleton, LocFun.add, LocFun.find. *)
+(*     destruct (Loc.eq_dec loc2 loc1); [congruence|]. *)
+(*     unfold LocFun.init. rewrite Cell.bot_join. auto. *)
+(*   } *)
+(*   i. des. *)
+(*   exploit Memory.write_future; try apply WRITE_SRC; eauto. *)
+(*   { apply WF1_SRC. } *)
+(*   { apply WF1_SRC. } *)
+(*   i. des. *)
+(*   exploit Memory.write_get; try apply WRITE_SRC; eauto. *)
+(*   { apply WF1_SRC. } *)
+(*   intro GET2_SRC. *)
+(*   exploit CommitFacts.write_min_spec; eauto. *)
+(*   { eapply Snapshot.writable_mon; [|apply COMMIT]. *)
+(*     etransitivity; [|apply COMMIT2]. apply COMMIT1. *)
+(*   } *)
+(*   { etransitivity; [apply COMMIT1|]. *)
+(*     etransitivity; [apply COMMIT2|]. *)
+(*     etransitivity; [apply COMMIT|]. apply COMMIT. *)
+(*   } *)
+(*   { instantiate (1 := ord2). inv COMMIT. i. *)
+(*     rewrite <- RELEASED, <- RELEASE; auto. *)
+(*     apply Snapshot.incr_writes_spec; auto. *)
+(*     etransitivity; [apply COMMIT1|]. *)
+(*     etransitivity; [apply COMMIT2|]. *)
+(*     apply MONOTONE. *)
+(*   } *)
+(*   { eapply Commit.future_wf; eauto. apply WF1_SRC. } *)
+(*   { inv WF2. exploit WF; eauto. } *)
+(*   i. des. *)
+(*   exploit Memory.le_get. *)
+(*   { apply WF1_SRC. } *)
+(*   { inv PROMISE. eapply Memory.le_get. *)
+(*     - apply Memory.le_join_r. memtac. *)
+(*     - apply Memory.singleton_get. *)
+(*   } *)
+(*   intro GET1_SRC. *)
+(*   exploit Memory.future_get; try apply GET1_SRC; eauto. *)
+(*   intro GET1_SRC'. *)
+(*   exploit CommitFacts.write_min_spec; try apply GET1_SRC'; eauto. *)
+(*   { eapply Snapshot.le_on_writable; eauto. apply COMMIT1. } *)
+(*   { inv COMMIT1. rewrite <- RELEASED, RELEASED1; auto. *)
+(*     apply MONOTONE. *)
+(*   } *)
+(*   { instantiate (1 := ord1). destruct ord1; ss. } *)
+(*   { inv WF2. exploit WF0; eauto. } *)
+(*   i. des. *)
+(*   eexists _, _. splits; eauto. *)
+(*   - econs; eauto. *)
+(*   - econs; eauto. s. *)
+(*     exploit CommitFacts.write_min_min; try apply COMMIT1; eauto. i. *)
+(*     exploit CommitFacts.write_min_min; try apply COMMIT; eauto. i. *)
+(*     inv x0. inv x1. *)
+(*     apply Snapshot.incr_writes_inv in CURRENT1. *)
+(*     apply Snapshot.incr_writes_inv in CURRENT2. des. *)
+(*     econs; ss. *)
+(*     + repeat apply Snapshot.incr_writes_spec; ss. *)
+(*       * etransitivity; [apply COMMIT1|]. *)
+(*         etransitivity; [apply COMMIT2|]. *)
+(*         apply COMMIT. *)
+(*       * etransitivity; [apply COMMIT1|]. *)
+(*         etransitivity; [apply COMMIT2|]. *)
+(*         apply COMMIT. *)
+(*     + i. unfold LocFun.add, LocFun.find. rewrite ORD1'. *)
+(*       etransitivity; [|apply RELEASED2]. *)
+(*       unfold LocFun.add, LocFun.find. *)
+(*       destruct (Loc.eq_dec loc loc1). *)
+(*       * subst. destruct (Loc.eq_dec loc1 loc2); [congruence|]. *)
+(*         etransitivity; [apply COMMIT1|]. apply COMMIT2. *)
+(*       * destruct (Loc.eq_dec loc loc2). *)
+(*         { subst. *)
+(*           match goal with *)
+(*           | [|- context[if ?c then _ else _]] => destruct c *)
+(*           end. *)
+(*           - apply Snapshot.join_spec. *)
+(*             + etransitivity; [|apply Snapshot.join_l]. *)
+(*               apply Snapshot.incr_writes_mon. *)
+(*               etransitivity; [apply COMMIT1|]. apply COMMIT2. *)
+(*             + etransitivity; [|apply Snapshot.join_r]. *)
+(*               etransitivity; [apply COMMIT1|]. apply COMMIT2. *)
+(*           - etransitivity; [apply COMMIT1|]. apply COMMIT2. *)
+(*         } *)
+(*         { etransitivity; [apply COMMIT1|]. apply COMMIT2. } *)
+(*     + etransitivity; [apply COMMIT1|]. *)
+(*       etransitivity; [apply COMMIT2|]. eauto. *)
+(* Qed. *)
